specify some in-place list map combinators

src/lowparse/steel_st_array/LowParse.SteelST.List.fst
@@ -1048,3 +1048,164 @@ let list_iter_opt
     rewrite (state _ _) (state res va.contents);
     return res
   end
+
+assume val list_map_inplace_le_opt
+  (#k: parser_kind)
+  (#t: Type)
+  (#p: parser k t)
+  (j: jumper p { k.parser_kind_subkind == Some ParserStrong })
+  (#k': parser_kind)
+  (#t': Type)
+  (p': parser k' t' { k.parser_kind_subkind == Some ParserStrong })
+  (phi: Ghost.erased (t -> t'))
+  (f: (
+    (va: v k t { AP.length (array_of' va) > 0 }) ->
+    (a: byte_array) ->
+    (vout: AP.v byte { AP.adjacent (AP.array_of vout) (array_of' va) }) -> // TODO: add write permissions
+    (out: byte_array) ->
+    STT SZ.size_t
+      (aparse p a va `star` AP.arrayptr out vout)
+      (fun res -> exists_ (fun res' -> exists_ (fun vres' -> exists_ (fun (vout': v _ _) ->
+        aparse p' out vout' `star` AP.arrayptr res' vres' `star` pure (
+        SZ.size_v res == AP.length (array_of vout') /\
+        SZ.size_v res > 0 /\
+        AP.merge_into (array_of' vout') (AP.array_of vres') (AP.merge (AP.array_of vout) (array_of' va)) /\
+        vout'.contents == Ghost.reveal phi va.contents
+      )))))
+  ))
+  (#va: _)
+  (a: byte_array)
+  (len: SZ.size_t { SZ.size_v len == length_opt va.array })
+  (#vout: _)
+  (out: byte_array { adjacent_opt (AP.array_of vout) va.array })  // TODO: add write permissions
+: STT SZ.size_t
+    (aparse_list p a va `star` AP.arrayptr out vout)
+    (fun res -> exists_ (fun res' -> exists_ (fun vres' -> exists_ (fun (vout': v _ _) ->
+      aparse (parse_list p') out vout' `star` AP.arrayptr res' vres' `star` pure (
+      SZ.size_v res == AP.length (array_of' vout') /\
+      AP.merge_into (array_of' vout') (AP.array_of vres') (merge_opt (AP.array_of vout) va.array) /\
+      vout'.contents == List.Tot.map phi va.contents
+    )))))
+
+#push-options "--z3rlimit 16"
+
+inline_for_extraction
+let list_map_inplace_le
+  (#k: parser_kind)
+  (#t: Type)
+  (#p: parser k t)
+  (j: jumper p { k.parser_kind_subkind == Some ParserStrong })
+  (#k': parser_kind)
+  (#t': Type)
+  (p': parser k' t' { k.parser_kind_subkind == Some ParserStrong })
+  (phi: Ghost.erased (t -> t'))
+  (f: (
+    (va: v k t { AP.length (array_of' va) > 0 }) ->
+    (a: byte_array) ->
+    (vout: AP.v byte { AP.adjacent (AP.array_of vout) (array_of' va) }) -> // TODO: add write permissions
+    (out: byte_array) ->
+    STT SZ.size_t
+      (aparse p a va `star` AP.arrayptr out vout)
+      (fun res -> exists_ (fun res' -> exists_ (fun vres' -> exists_ (fun (vout': v _ _) ->
+        aparse p' out vout' `star` AP.arrayptr res' vres' `star` pure (
+        SZ.size_v res == AP.length (array_of vout') /\
+        SZ.size_v res > 0 /\
+        AP.merge_into (array_of' vout') (AP.array_of vres') (AP.merge (AP.array_of vout) (array_of' va)) /\
+        vout'.contents == Ghost.reveal phi va.contents
+      )))))
+  ))
+  (#va: _)
+  (a: byte_array)
+  (len: SZ.size_t { SZ.size_v len == AP.length (array_of' va) })
+  (#vout: _)
+  (out: byte_array { AP.adjacent (AP.array_of vout) (array_of' va) })  // TODO: add write permissions
+: STT SZ.size_t
+    (aparse (parse_list p) a va `star` AP.arrayptr out vout)
+    (fun res -> exists_ (fun res' -> exists_ (fun vres' -> exists_ (fun (vout': v _ _) ->
+      aparse (parse_list p') out vout' `star` AP.arrayptr res' vres' `star` pure (
+      SZ.size_v res == AP.length (array_of' vout') /\
+      AP.merge_into (array_of' vout') (AP.array_of vres') (AP.merge (AP.array_of vout) (array_of' va)) /\
+      vout'.contents == List.Tot.map phi va.contents
+    )))))
+= intro_aparse_list p out a;
+  let _ = gen_elim () in
+  let res = list_map_inplace_le_opt j p' phi f a len out in
+  let _ = gen_elim () in
+  return res
+
+#pop-options
+
+assume val list_map_inplace_eq_opt
+  (#k: parser_kind)
+  (#t: Type)
+  (#p: parser k t)
+  (j: jumper p { k.parser_kind_subkind == Some ParserStrong })
+  (#k': parser_kind)
+  (#t': Type)
+  (p': parser k' t' { k.parser_kind_subkind == Some ParserStrong })
+  (phi: Ghost.erased (t -> t'))
+  (f: (
+    (va: v k t { AP.length (array_of' va) > 0 }) -> // TODO: add write permissions
+    (a: byte_array) ->
+    STT (v k' t')
+      (aparse p a va)
+      (fun va' -> aparse p' a va' `star` pure (
+        array_of' va' == array_of' va /\
+        va'.contents == Ghost.reveal phi va.contents
+      ))
+  ))
+  (#va: _)
+  (a: byte_array)
+  (len: SZ.size_t)
+: ST _
+    (aparse_list p a va)
+    (fun va' -> aparse_list p' a va')
+    (SZ.size_v len == length_opt va.array)  // TODO: add write permissions
+    (fun va' ->
+      va'.array == va.array /\
+      va'.contents == List.Tot.map phi va.contents
+    )
+
+inline_for_extraction
+let list_map_inplace_eq
+  (#k: parser_kind)
+  (#t: Type)
+  (#p: parser k t)
+  (j: jumper p { k.parser_kind_subkind == Some ParserStrong })
+  (#k': parser_kind)
+  (#t': Type)
+  (p': parser k' t' { k.parser_kind_subkind == Some ParserStrong })
+  (phi: Ghost.erased (t -> t'))
+  (f: (
+    (va: v k t { AP.length (array_of' va) > 0 }) -> // TODO: add write permissions
+    (a: byte_array) ->
+    STT (v k' t')
+      (aparse p a va)
+      (fun va' -> aparse p' a va' `star` pure (
+        array_of' va' == array_of' va /\
+        va'.contents == Ghost.reveal phi va.contents
+      ))
+  ))
+  (#va: v _ _)
+  (a: byte_array)
+  (len: SZ.size_t)
+: ST (v _ _)
+    (aparse (parse_list p) a va)
+    (fun va' -> aparse (parse_list p') a va')
+    (SZ.size_v len == AP.length (array_of' va))  // TODO: add write permissions
+    (fun va' ->
+      array_of' va' == array_of' va /\
+      va'.contents == List.Tot.map phi va.contents
+    )
+= let _ = ghost_is_cons p a in
+  if len = SZ.zero_size
+  then begin
+    let _ = elim_nil p a in
+    let res = intro_nil p' a in
+    return res
+  end else begin
+    let _ = intro_aparse_list_cons p a _ in
+    let _ = list_map_inplace_eq_opt j p' phi f a len in
+    let res = elim_aparse_list_cons p' a _ in
+    return res
+  end
